soundness comes first

src/coq/dot/meta_inversion.v
@@ -4,6 +4,27 @@ Require Import syntax_binding theory.
 Require Import Metatheory LibTactics_sf support meta_regular meta_binding.
 Require Import Coq.Program.Equality.
 
+
+(**
+  [gen_eq c as x H] takes all occurrences of [c] in the current goal's
+  conclusion, replaces them by the variable [x], and introduces the equality
+  [x = c] as the hypothesis H.  Useful if one needs to generalize the goal
+  prior to applying an induction tactic.
+*)
+
+Tactic Notation "gen_eq" constr(c) "as" ident(x) ident(H) :=
+  set (x := c); assert (H : x = c) by reflexivity; clearbody x.
+
+(**
+  A variation on the above in which all occurrences of [c] in the goal are
+  replaced, not only those in the conclusion.
+*)
+
+Tactic Notation "gen_eq" constr(c) "as" ident(x) :=
+  set (x := c) in *;
+  let H := fresh in (assert (H : x = c) by reflexivity; clearbody x; revert H).
+
+
 (* FAILED attempts at inversion lemma for subtyping of function types:
 
 (1)
@@ -55,8 +76,10 @@ prove soundness and completeness wrt the original relations (where expansion has
 Reserved Notation "E |= t ~<! T" (at level 69).
 
 (*
-subtyping from a parallel universe where transitivity is unheard of; also, to simplify the proof, expansion and sub_decl are rolled into subtyping, and quality is glossed over, since inversion doesn't need to preserve quality
-(and inversion is why we have sub_tp_notrans in the first place -- you try inverting something with an explicit rule for transivity some time)
+subtyping from a parallel universe where transitivity is unheard of; also, to simplify the proof, expansion and sub_decl are rolled into subtyping,
+and quality is glossed over (need to improve my Ltac-f to bring it back: existentials must be crushed, qualities normalised), 
+since inversion doesn't need to preserve quality this is not urgent, though
+(inversion is why we have sub_tp_notrans in the first place -- you try inverting something with an explicit rule for transivity some time)
 
 the order of the rules, and especially the order of the hypotheses in sub_tp_notrans_rfn_r is tuned for eauto 
 as used in the proof of transitivity, sub_tp_notrans_trans (more constraining hypotheses come first) 
@@ -84,13 +107,6 @@ Inductive sub_tp_notrans : env -> tp -> tp -> Prop :=
       and_decls DSP DS DS1 ->
       E |= T ~<! (tp_rfn Tpar DS) -> E |= Tpar ~<! (tp_rfn tp_top DSP) ->  (* was E |= T ~< DS1 *)
       E |= T ~<! (tp_rfn T' DS2) 
-
-(* subsumed by sub_tp_notrans_rfn_r 
-   | expands_rfn : forall E Tpar DSP DS DSM,
-      E |= T ~<! (tp_rfn Tpar DS) ->
-      E |= Tpar ~<! (tp_rfn tp_top DSP) -> and_decls DSP DS DSM ->
-      E |= T ~<! (tp_rfn tp_top DSM) *)
-
 
   | sub_tp_notrans_and_r : forall E T T1 T2,
       E |= T ~<! T1 -> E |= T ~<! T2 ->
@@ -130,7 +146,6 @@ Inductive sub_tp_notrans : env -> tp -> tp -> Prop :=
   | sub_tp_notrans_and_l1 : forall E T T1 T2,
       E |= T1 ~<! T -> 
       E |= (tp_and T1 T2) ~<! T
-
   | sub_tp_notrans_and_l2 : forall E T T1 T2,
       E |= T2 ~<! T -> 
       E |= (tp_and T1 T2) ~<! T  
@@ -139,7 +154,7 @@ Inductive sub_tp_notrans : env -> tp -> tp -> Prop :=
       E |= T1 ~<! T -> E |= T2 ~<! T ->
       E |= (tp_or T1 T2) ~<! T
 
-  | sub_tp_notrans_bot  : forall E T, E |= tp_bot ~<! T
+  | sub_tp_notrans_bot  : forall E T, E |= tp_bot ~<! T (* hide bottom down here, where it belongs *)
 
 where "E |= T1 ~<! T2" := (sub_tp_notrans E T1 T2).
 
@@ -153,33 +168,122 @@ Definition sub_decls_under L E T DS1 DS2 :=
 
 
 
-Section NoTransSoundComplete.
-
-
-Tactic Notation "gen_eq" constr(c) "as" ident(x) ident(H) :=
-  set (x := c); assert (H : x = c) by reflexivity; clearbody x.
-
 Hint Constructors sub_tp_notrans.
 (*Hint Resolve sub_tp_notrans_fun sub_tp_notrans_tpsel_r sub_tp_notrans_rfn_r expands_rfn sub_tp_notrans_and_r expands_and sub_tp_notrans_or_r1 sub_tp_notrans_or_r2 expands_or sub_tp_notrans_refl sub_tp_notrans_top expands_top sub_tp_notrans_tpsel_l sub_tp_notrans_rfn_l sub_tp_notrans_and_l1 sub_tp_notrans_and_l2 sub_tp_notrans_or_l. *)
 
-(*
-rename t into p. rename T into Ta. rename T0 into Tb. rename T'0 into T.
-rename DS0 into DS'. rename S0 into S'. rename U0 into U'.
-clear IHHSubR1 IHHSubR2 IHHSubL1 IHHSubL2.
+Section Soundness.
+  (* TODO: deal with regularity  *)
+  Lemma wf_ax : forall E, wf_env E. Proof. Admitted.
+  Lemma lc_ax : forall T, lc_tp T. Proof. Admitted.
+  Hint Resolve wf_ax lc_ax.
 
-  H : path_safe E p
-  H4 : E |= p ~: T' @ q0
-  HSubR1 : E |= T' ~<! tp_rfn tp_top DS'
-  H2 : lbl.binds l (decl_tp S' U') DS'
-  HSubR2 : E |= U' ^tp^ p ~<! Tb
+  Hint Constructors expands.
+  Hint Resolve sub_tp_rfn sub_tp_rfn_elim sub_tp_tpsel_lower sub_tp_tpsel_upper sub_tp_refl sub_tp_top sub_tp_bot sub_tp_fun sub_tp_and_r sub_tp_or_l sub_tp_and_l1 sub_tp_and_l2 sub_tp_or_r1 sub_tp_or_r2. (*but not transitivity*)
 
-  H0 : E |= p ~: T @ q1
-  HSubL1 : E |= T ~<! tp_rfn tp_top DS
-  H1 : lbl.binds l (decl_tp S U) DS
-  HSubL2 : E |= Ta ~<! S ^tp^ p
+  Lemma and_decls_nil: and_decls nil nil nil.            Proof. Admitted.
+  Lemma and_decls_nil_1: forall DS, and_decls nil DS DS. Proof. Admitted.
+  Lemma and_decls_nil_2: forall DS, and_decls DS nil DS. Proof. Admitted.
+  Lemma or_decls_nil: or_decls nil nil nil.              Proof. Admitted.
+  Lemma or_decls_nil_1: forall DS, or_decls nil DS nil.  Proof. Admitted.
+  Lemma or_decls_nil_2: forall DS, or_decls DS nil nil.  Proof. Admitted.
 
-eapply sub_tp_notrans_trans_tpsel with (T' := T'); eauto.
-*)
+  (* TODO: proof will need decls_ok from well formedness of the type that expanded to DS *)
+  Lemma sub_decls_refl : forall L E DS qs T,
+     forall z : atom, z `notin` L -> forall (l : label) (d2 : decl), lbl.binds l d2 DS -> exists d1, lbl.binds l d1 DS /\ 
+     (exists q, In q qs /\ sub_decl (ctx_bind E z T) q (d1 ^d^ z) (d2 ^d^ z)).
+  Proof. Admitted.
+
+  Hint Resolve and_decls_nil and_decls_nil_1 and_decls_nil_2 or_decls_nil or_decls_nil_1 or_decls_nil_2 sub_decls_refl.
+
+  (* specialize hypotheses with satisfiable embedded equalities, drop the unsatisfiable ones *)
+  Ltac sphyps :=
+    repeat match goal with H: ?T |- _ => 
+      match T with
+      | forall x, ?a = _ -> _  => 
+        match type of a with
+          | ?x => try (let h := fresh in lets h: H (@eq_refl x); generalizes h); clear H
+        end
+      | _ => generalizes H
+      end
+    end.
+  Ltac simplhyps :=  jauto_set_hyps; intros; sphyps; intros; jauto_set_hyps; intros.
+
+  (* TODO: how do we expose the subtyping judgements in sub_decls, so that we get an IH??
+   (forall z : atom,
+         z `notin` L ->
+         forall (l : label) (d2 : decl),
+         lbl.binds l d2 DS0 ->
+         exists d1,
+         lbl.binds l d1 DS1 /\
+         (forall S1 T1 S2 T2 : tp,
+          d1 ^d^ z = decl_tp S1 T1 /\ d2 ^d^ z = decl_tp S2 T2 ->
+          ctx_bind E z T |= S2 ~<! S1 /\ ctx_bind E z T |= T1 ~<! T2) /\
+         (forall T1 T2 : tp,
+          d1 ^d^ z = decl_tm T1 /\ d2 ^d^ z = decl_tm T2 ->
+          ctx_bind E z T |= T1 ~<! T2)) ->
+     (exists qs, forall z : atom,
+     z `notin` L ->
+     forall (l : label) (d2 : decl),
+     lbl.binds l d2 DS0 ->
+     exists d1,
+     lbl.binds l d1 DS1 /\
+     (exists q,
+      In q qs /\
+      sub_decl (ctx_bind E z (tp_rfn Tpar DS)) q (d1 ^d^ z) (d2 ^d^ z)))
+
+  *)
+  Lemma notrans_is_sound : forall E T1 T2, E |= T1 ~<! T2 -> (exists q, E |= T1 ~<: T2 @ q) /\ 
+    (forall DS, T2 = tp_rfn tp_top DS -> exists q, E |= T1 ~< DS @ q). 
+  Proof. 
+    introv H. gen E T1 T2.
+     dependent induction H; (split; [ 
+       simplhyps; eauto 3 | (* subtyping *)
+       introv HEq; try injsubst HEq; subst;  (* expansion *)
+         try destructs IHsub_tp_notrans1; try destructs IHsub_tp_notrans2; try destructs IHsub_tp_notrans; 
+         simplhyps; try solve [ discriminate | eexists; intros; eauto 3] ]).
+
+    eexists; eapply sub_tp_trans with (TMid := S ^tp^ p); eauto.
+
+    eexists; eapply sub_tp_rfn with (DS1 := DS1) (DS2 := DS2) (qs := subsumed :: nil) (q := subsumed); eauto 3. 
+    skip. (* TODO: IH for sub_decls *)
+    intros; discriminate.
+
+    forwards: (@sub_tp_rfn L E T tp_top DS1 DS0 (x & x1) subsumed (subsumed :: nil) subsumed); eauto 3.
+    skip. (* TODO: IH for sub_decls *)
+    intros. discriminate.
+    
+    eexists; eauto.
+
+    Ltac sub_tp_rfn_top DS := eapply sub_tp_rfn with (DS1 := DS) (DS2 := DS) (qs := subsumed :: nil) (q := subsumed); eauto; intros; discriminate.
+
+    eexists; eapply sub_tp_trans with (TMid := tp_and T1 T2); [ eauto | sub_tp_rfn_top DSM].
+
+    eexists; eapply sub_tp_trans with (TMid := T1); eauto.
+
+    eexists; eapply sub_tp_trans with (TMid := T2); eauto.
+
+    eexists; eapply sub_tp_trans with (TMid := tp_or T1 T2); [eauto | sub_tp_rfn_top DSM].
+
+    eexists; sub_tp_rfn_top (nil : decls).
+
+    eexists; eapply sub_tp_trans with (TMid := U ^tp^ p); eauto.
+
+    eexists; eapply sub_tp_trans with (TMid := T); eauto. 
+
+    eexists; eapply sub_tp_trans with (TMid := T1); eauto. 
+
+    eexists; eapply sub_tp_trans with (TMid := T2); eauto. 
+
+    eexists; eapply expands_sub with (U := tp_rfn tp_top DS); eauto. 
+
+    admit. (* TODO: the old system does not have an explicit rule to expand tp_bot since expands_sub subsumes to any supertype that has an expansion *)
+
+  Admitted.
+End Soundness.
+
+
+
+
 
 (* no way this can be a rule -- the transitivity proof peterait un plomb 
 
@@ -201,9 +305,45 @@ Lemma sub_tp_notrans_trans_tpsel : forall E q1 q2 p T DS l S U T' DS' S' U' Ta T
 
   E |= Ta ~<! Tb.
 Proof. Admitted.
+(*
+rename t into p. rename T into Ta. rename T0 into Tb. rename T'0 into T.
+rename DS0 into DS'. rename S0 into S'. rename U0 into U'.
+clear IHHSubR1 IHHSubR2 IHHSubL1 IHHSubL2.
 
-(* TODO: T well-formedness/kindedness hypotheses? *)
-Lemma strengthen_sub_decls: forall L E S T DS1 DS2,  
+  H : path_safe E p
+  H4 : E |= p ~: T' @ q0
+  HSubR1 : E |= T' ~<! tp_rfn tp_top DS'
+  H2 : lbl.binds l (decl_tp S' U') DS'
+  HSubR2 : E |= U' ^tp^ p ~<! Tb
+
+  H0 : E |= p ~: T @ q1
+  HSubL1 : E |= T ~<! tp_rfn tp_top DS
+  H1 : lbl.binds l (decl_tp S U) DS
+  HSubL2 : E |= Ta ~<! S ^tp^ p
+
+eapply sub_tp_notrans_trans_tpsel with (T' := T'); eauto.
+*)
+
+
+
+Definition transitivity_on TMid := forall E T T',  E |= T ~<! TMid -> E |= TMid ~<! T' -> E |= T ~<! T'.
+Hint Unfold transitivity_on.
+
+Lemma sub_narrowing_aux : forall TMid s F E z Sz Tz S T,
+  transitivity_on TMid ->
+  (E ++ z ~ (Tz, (precise, true)) ++ F, s) |= S ~<! T ->
+  (E, s) |= Sz ~<! Tz ->
+  (E ++ z ~ (Sz, (precise, true)) ++ F, s) |= S ~<! T.
+Proof.
+  introv HTrans HSubL HSubZ.
+  gen_eq (E ++ z ~ (Tz, (precise, true)) ++ F, s) as G. gen F.
+  induction HSubL; introv EQ; subst; eauto 5.
+
+  eapply sub_tp_notrans_tpsel_r; eauto. eapply typing_sub with (S := T').
+  skip. eapply IHHSubL2; eauto.
+
+
+Lemma narrow_sub_decls: forall L E S T DS1 DS2,  
      (forall z, z \notin L -> (forall l d2, lbl.binds l d2 DS2 -> exists d1, lbl.binds l d1 DS1 /\
            (forall S1 T1 S2 T2, ((d1 ^d^ z) = (decl_tp S1 T1) /\ (d2 ^d^ z) = (decl_tp S2 T2)) -> 
               (ctx_bind E z T) |= S2 ~<! S1 /\ (ctx_bind E z T) |= T1 ~<! T2 ) /\
@@ -219,28 +359,28 @@ Lemma strengthen_sub_decls: forall L E S T DS1 DS2,
           )).
 Proof. Admitted.
 
-Hint Resolve strengthen_sub_decls.
+Hint Resolve narrow_sub_decls.
+
 
 (* inspired by sub_transitivity from http://www.chargueraud.org/arthur/research/2007/binders/src/Fsub_Soundness.html
 
   Coq provides "dependent induction" to perform "Induction/inversion principle"; 4.2.1. of
    http://www.msr-inria.inria.fr/~gares/jar09.pdf explains the latter is needed to perform a proof like this
 *)
-Lemma sub_tp_notrans_trans : forall E T TMid T',
-  E |= T ~<! TMid -> E |= TMid ~<! T' -> E |= T ~<! T'.
+Lemma sub_tp_notrans_trans : forall TMid, transitivity_on TMid.
 Proof.
  introv HSubL HSubR. gen E T T'. gen_eq TMid as TMid' eq. gen TMid' eq. 
  induction TMid; intros TMid' EQ; intros;
    dependent induction HSubL; try discriminate; inversions EQ;
      intros; dependent induction HSubR; subst; auto; try solve [ 
-       eapply sub_tp_notrans_rfn_r; eauto 2; eapply strengthen_sub_decls; eauto 2 |
+       eapply sub_tp_notrans_rfn_r; eauto 2; eapply narrow_sub_decls; eauto 2 |
        eapply sub_tp_notrans_and_r; eauto 2 | 
        eapply sub_tp_notrans_and_l1; eapply IHHSubL; eauto 2 |
        eapply sub_tp_notrans_and_l2; eapply IHHSubL; eauto 2 |
        eapply sub_tp_notrans_rfn_l; eapply IHHSubL; eauto 2 |
        eapply sub_tp_notrans_tpsel_l; eauto 3 using sub_tp_notrans_rfn_r |
        eapply sub_tp_notrans_or_l; eauto 3 using IHHSubL1, sub_tp_notrans_tpsel_l, IHHSubL2 |
-       eapply sub_tp_notrans_rfn_r; eauto 3 using IHHSubR1, strengthen_sub_decls, sub_tp_notrans_rfn_r, IHHSubR2 |
+       eapply sub_tp_notrans_rfn_r; eauto 3 using IHHSubR1, narrow_sub_decls, sub_tp_notrans_rfn_r, IHHSubR2 |
        eapply sub_tp_notrans_fun; eauto 2 using IHTMid1, IHTMid2 |
        eauto 3]. (* less than 2 minutes*)
 
@@ -303,171 +443,45 @@ Lemma invert_fun_notrans : forall E Sa Sr Ta Tr,
   E |= Ta ~<! Sa  /\  E |= Sr ~<! Tr.
 Proof.
 intros.
-(*assert (wf_env E) by admit. assert (lc_tp Ta) by admit. assert (lc_tp Tr) by admit.*)
 inverts H; splits; auto. 
 Qed.
 
-Section Soundness.
- (* TODO: deal with regularity  *)
-Lemma wf_ax : forall E, wf_env E. Proof. Admitted.
-Lemma lc_ax : forall T, lc_tp T. Proof. Admitted.
-Hint Resolve wf_ax lc_ax.
 
-Hint Constructors expands.
-Hint Resolve sub_tp_rfn sub_tp_rfn_elim sub_tp_tpsel_lower sub_tp_tpsel_upper sub_tp_refl sub_tp_top sub_tp_bot sub_tp_fun sub_tp_and_r sub_tp_or_l sub_tp_and_l1 sub_tp_and_l2 sub_tp_or_r1 sub_tp_or_r2. (*but not transitivity*)
-
-Lemma and_decls_nil: and_decls nil nil nil.
-Proof. Admitted.
-
-Lemma and_decls_nil_1: forall DS, and_decls nil DS DS.
-Proof. Admitted.
-
-Lemma and_decls_nil_2: forall DS, and_decls DS nil DS.
-Proof. Admitted.
-
-Lemma or_decls_nil: or_decls nil nil nil.
-Proof. Admitted.
-
-Lemma or_decls_nil_1: forall DS, or_decls nil DS nil.
-Proof. Admitted.
-
-Lemma or_decls_nil_2: forall DS, or_decls DS nil nil.
-Proof. Admitted.
-
-Lemma sub_decls_refl : forall L E DS qs T,
-   forall z : atom,
-   z `notin` L ->
-   forall (l : label) (d2 : decl),
-   lbl.binds l d2 DS ->
-   exists d1,
-   lbl.binds l d1 DS /\
-   (exists q,
-    In q qs /\
-    sub_decl (ctx_bind E z T) q (d1 ^d^ z) (d2 ^d^ z)).
-Proof. Admitted.
-
-Hint Resolve and_decls_nil and_decls_nil_1 and_decls_nil_2 or_decls_nil or_decls_nil_1 or_decls_nil_2 sub_decls_refl.
-
-(* specialize hypotheses with satisfiable embedded equalities, drop the unsatisfiable ones *)
-Ltac shyps :=
-  repeat match goal with H: ?T |- _ => 
-    match T with
-    | forall x, ?a = _ -> _  => 
-      match type of a with
-        | ?x => try (let h := fresh in lets h: H (@eq_refl x); generalizes h); clear H
-      end
-    | _ => generalizes H
-    end
-  end.
-
-Ltac simplhyps :=  jauto_set_hyps; intros; shyps; intros; jauto_set_hyps; intros.
-
-Ltac sub_tp_rfn_top DS := eapply sub_tp_rfn with (DS1 := DS) (DS2 := DS) (qs := subsumed :: nil) (q := subsumed); eauto; intros; discriminate.
-
-(*
- (forall z : atom,
-       z `notin` L ->
-       forall (l : label) (d2 : decl),
-       lbl.binds l d2 DS0 ->
-       exists d1,
-       lbl.binds l d1 DS1 /\
-       (forall S1 T1 S2 T2 : tp,
-        d1 ^d^ z = decl_tp S1 T1 /\ d2 ^d^ z = decl_tp S2 T2 ->
-        ctx_bind E z T |= S2 ~<! S1 /\ ctx_bind E z T |= T1 ~<! T2) /\
-       (forall T1 T2 : tp,
-        d1 ^d^ z = decl_tm T1 /\ d2 ^d^ z = decl_tm T2 ->
-        ctx_bind E z T |= T1 ~<! T2)) ->
-   (exists qs, forall z : atom,
-   z `notin` L ->
-   forall (l : label) (d2 : decl),
-   lbl.binds l d2 DS0 ->
-   exists d1,
-   lbl.binds l d1 DS1 /\
-   (exists q,
-    In q qs /\
-    sub_decl (ctx_bind E z (tp_rfn Tpar DS)) q (d1 ^d^ z) (d2 ^d^ z)))
-
-*)
-Lemma notrans_is_sound : forall E T1 T2, E |= T1 ~<! T2 -> (exists q, E |= T1 ~<: T2 @ q) /\ 
-  (forall DS, T2 = tp_rfn tp_top DS -> exists q, E |= T1 ~< DS @ q). 
-Proof. 
-introv H. gen E T1 T2.
- dependent induction H; (split; [ 
-   simplhyps; eauto 3 |
-   introv HEq; try injsubst HEq; subst; try destructs IHsub_tp_notrans1; try destructs IHsub_tp_notrans2; try destructs IHsub_tp_notrans; simplhyps; try solve [ discriminate | eexists; intros; eauto 3]]).
-
-eexists; eapply sub_tp_trans with (TMid := S ^tp^ p); eauto.
-
-eexists; eapply sub_tp_rfn with (DS1 := DS1) (DS2 := DS2) (qs := subsumed :: nil) (q := subsumed); eauto 3. 
-skip. (* TODO: IH for sub_decls *)
-intros; discriminate.
-
-forwards: (@sub_tp_rfn L E T tp_top DS1 DS0 (x & x1) subsumed (subsumed :: nil) subsumed); eauto 3.
-skip. (* TODO: IH for sub_decls *)
-intros. discriminate.
-eexists; eauto.
-
-eexists; eapply sub_tp_trans with (TMid := tp_and T1 T2); [ eauto | sub_tp_rfn_top DSM].
-
-eexists; eapply sub_tp_trans with (TMid := T1); eauto.
-
-eexists; eapply sub_tp_trans with (TMid := T2); eauto.
-
-eexists; eapply sub_tp_trans with (TMid := tp_or T1 T2); [eauto | sub_tp_rfn_top DSM].
-
-eexists; sub_tp_rfn_top (nil : decls).
-
-eexists; eapply sub_tp_trans with (TMid := U ^tp^ p); eauto.
-
-eexists; eapply sub_tp_trans with (TMid := T); eauto. 
-
-eexists; eapply sub_tp_trans with (TMid := T1); eauto. 
-
-eexists; eapply sub_tp_trans with (TMid := T2); eauto. 
-
-eexists; eapply expands_sub with (U := tp_rfn tp_top DS); eauto. 
-
-admit. (* TODO: there's no actual rule to expand tp_bot, instead use expands_sub to whatever subtype that has an expansion *)
-
-Admitted.
-
-End Soundness.
 
 
 Section Completeness.
 
-  Let P2_ (E : env) (q : quality) (S T : tp) (H: E |= S ~<: T @ q) := E |= S ~<! T.
-  Let P1_ (E : env) (q : quality) (T : tp) (DS : decls) (H: E |= T ~< DS @ q) := E |= T ~<! tp_rfn tp_top DS.
+    Let P2_ (E : env) (q : quality) (S T : tp) (H: E |= S ~<: T @ q) := E |= S ~<! T.
+    Let P1_ (E : env) (q : quality) (T : tp) (DS : decls) (H: E |= T ~< DS @ q) := E |= T ~<! tp_rfn tp_top DS.
 
-  Let P0_ (E_s: env) (q: quality) (t: tm) (T: tp) (H: E_s |=  t ~: T  @ q) := True.
-  Let P3_ (e : env) (q : quality) (d d0 : decl) (H: sub_decl e q d d0) := True.
-  Let P4_ (e : env) (t t0 : tm) (H: path_eq e t t0) := True.
-  Let P5_ (e : env) (H: wf_env e) := True.
-  Let P6_ (e : env) (t : tp) (H: wf_tp e t) := True.
-  Let P7_ (e : env) (d : decl) (H: wf_decl e d) := True.
+    Let P0_ (E_s: env) (q: quality) (t: tm) (T: tp) (H: E_s |=  t ~: T  @ q) := True.
+    Let P3_ (e : env) (q : quality) (d d0 : decl) (H: sub_decl e q d d0) := True.
+    Let P4_ (e : env) (t t0 : tm) (H: path_eq e t t0) := True.
+    Let P5_ (e : env) (H: wf_env e) := True.
+    Let P6_ (e : env) (t : tp) (H: wf_tp e t) := True.
+    Let P7_ (e : env) (d : decl) (H: wf_decl e d) := True.
 
-(* only hard case is sub_tp_trans, which is proven above *)
-Lemma notrans_is_complete : (forall E q S T, E |= S ~<: T @ q -> E |= S ~<! T) /\ (forall E q T DS, E |= T ~< DS @ q -> E |= T ~<! tp_rfn tp_top DS).
-Proof.
-  cut ((forall E q t T (H: E |= t ~: T @ q), (@P0_ E q t T H)) /\ 
-  (forall E q T DS (H: E |= T ~< DS @ q), (@P1_ E q T DS H)) /\ 
-  (forall E q T T' (H: E |= T ~<: T' @ q), (@P2_  E q T T' H))  /\ 
-  (forall (e : env) (q : quality) (d d0 : decl) (H : sub_decl e q d d0), (@P3_ e q d d0 H)) /\  
-  (forall (e : env) (t t0 : tm) (H : path_eq e t t0), (@P4_ e t t0 H)) /\  
-  (forall (e : env) (H : wf_env e), (@P5_ e H)) /\
-  (forall (e : env) (t : tp) (H : wf_tp e t), (@P6_ e t H)) /\  
-  (forall (e : env) (d : decl) (H : wf_decl e d), (@P7_ e d H))); [tauto | 
-    apply (typing_mutind P0_ P1_ P2_ P3_ P4_ P5_ P6_ P7_); unfold P0_, P1_, P2_, P3_, P4_, P5_, P6_, P7_ in *; clear P0_ P1_ P2_ P3_ P4_ P5_ P6_ P7_]; intros; eauto 3. 
+  (* only hard case is sub_tp_trans, which is proven above *)
+  Lemma notrans_is_complete : (forall E q S T, E |= S ~<: T @ q -> E |= S ~<! T) /\ (forall E q T DS, E |= T ~< DS @ q -> E |= T ~<! tp_rfn tp_top DS).
+  Proof.
+    cut ((forall E q t T (H: E |= t ~: T @ q), (@P0_ E q t T H)) /\ 
+    (forall E q T DS (H: E |= T ~< DS @ q), (@P1_ E q T DS H)) /\ 
+    (forall E q T T' (H: E |= T ~<: T' @ q), (@P2_  E q T T' H))  /\ 
+    (forall (e : env) (q : quality) (d d0 : decl) (H : sub_decl e q d d0), (@P3_ e q d d0 H)) /\  
+    (forall (e : env) (t t0 : tm) (H : path_eq e t t0), (@P4_ e t t0 H)) /\  
+    (forall (e : env) (H : wf_env e), (@P5_ e H)) /\
+    (forall (e : env) (t : tp) (H : wf_tp e t), (@P6_ e t H)) /\  
+    (forall (e : env) (d : decl) (H : wf_decl e d), (@P7_ e d H))); [tauto | 
+      apply (typing_mutind P0_ P1_ P2_ P3_ P4_ P5_ P6_ P7_); unfold P0_, P1_, P2_, P3_, P4_, P5_, P6_, P7_ in *; clear P0_ P1_ P2_ P3_ P4_ P5_ P6_ P7_]; intros; eauto 3. 
 
-apply sub_tp_notrans_trans with (TMid := U); eauto.
-eapply sub_tp_notrans_rfn_r; eauto. 
-skip. (* TODO: sub_decl_refl *)
-eapply sub_tp_notrans_rfn_r with (DS1 := DS1); eauto. 
-skip. (* TODO: IH for sub_Decls *)
-apply and_decls_nil_1.
-apply sub_tp_notrans_trans with (TMid := TMid); eauto.
-
-Qed.
+    apply sub_tp_notrans_trans with (TMid := U); eauto.
+    eapply sub_tp_notrans_rfn_r; eauto. 
+    skip. (* TODO: sub_decl_refl *)
+    eapply sub_tp_notrans_rfn_r with (DS1 := DS1); eauto. 
+    skip. (* TODO: IH for sub_decls *)
+    apply and_decls_nil_1.
+    apply sub_tp_notrans_trans with (TMid := TMid); eauto.
+  Qed.
 
 End NoTransSoundComplete.
 
@@ -536,325 +550,6 @@ Lemma invert_red_store_dom : forall s t t' s', s |~ t ~~> t' ~| s' -> dom s [<=]
 Proof. Admitted.
 
 
-
-
-
-
-
-
-
-
-
-
-
-
-
-
-
-
-
-
-
-
-
-
-(* doesn't work:
-  case := "sub_tp_trans" : String.string
-  E : env
-  q1 : quality
-  q2 : quality
-  TMid : tp
-  T : tp
-  n : forall (p : tm) (L : label), TMid <> tp_sel p L
-  s : E |= T ~<: TMid @ q1
-  H : forall T1 T2 : tp,
-      TMid = tp_fun T1 T2 ->
-      (exists p L, T = tp_sel p L) \/
-      (exists T3 T4, T = tp_and T3 T4) \/
-      (exists T3 T4, T = tp_or T3 T4) \/
-      (exists TP DS, T = tp_rfn TP DS) \/
-      (exists T1' T2',
-       T = tp_fun T1' T2' ->
-       exists q, E |= T1 ~<: T1' @ q /\ (exists q0, E |= T2' ~<: T2 @ q0))
-  T1 : tp
-  T2 : tp
-  s0 : E |= TMid ~<: tp_fun T1 T2 @ q2
-  H0 : forall T3 T4 : tp,
-       tp_fun T1 T2 = tp_fun T3 T4 ->
-       (exists p L, TMid = tp_sel p L) \/
-       (exists T1 T2, TMid = tp_and T1 T2) \/
-       (exists T1 T2, TMid = tp_or T1 T2) \/
-       (exists TP DS, TMid = tp_rfn TP DS) \/
-       (exists T1' T2',
-        TMid = tp_fun T1' T2' ->
-        exists q, E |= T3 ~<: T1' @ q /\ (exists q0, E |= T2' ~<: T4 @ q0))
-  ============================
-   exists T1' T2',
-   T = tp_fun T1' T2' ->
-   exists q, E |= T1 ~<: T1' @ q /\ (exists q0, E |= T2' ~<: T2 @ q0)
-
-
-Section InvSubFun0.
-  Let P0_ (E: env) (q: quality) (t: tm) (T: tp) (H: E  |=  t ~: T  @ q) := True.  Let P3_ (e : env) (q : quality) (d d0 : decl) (H: sub_decl e q d d0) := True.  Let P4_ (e : env) (t t0 : tm) (H: path_eq e t t0) := True.  Let P5_ (e : env) (H: wf_env e) := True. Let P6_ (e : env) (t : tp) (H: wf_tp e t) := True.  Let P7_ (e : env) (d : decl) (H: wf_decl e d) := True.
-
-
-  Let P1_ (E : env) (q : quality) (T : tp) (DS : decls) (H: E |= T ~< DS @ q) := forall T1 T2, T = tp_fun T1 T2 -> 
-    DS = nil.
-  Let P2_ (E : env) (q : quality) (S T : tp) (H: E |= S ~<: T @ q) := forall T1 T2, T = tp_fun T1 T2 -> 
-    (exists p, exists L, S = tp_sel p L) \/ (exists T1, exists T2, S = tp_and T1 T2) \/ (exists T1, exists T2, S = tp_or T1 T2) \/ (exists TP, exists DS, S = tp_rfn TP DS) \/ 
-    (exists T1', exists T2', S = tp_fun T1' T2' -> exists q, E |= T1 ~<: T1' @ q /\ exists q, E |= T2' ~<: T2 @ q ).
-
-
-Lemma invert_subtyping_fun0 : 
-   (forall E q T DS, E |= T ~< DS @ q -> forall T1 T2, T = tp_fun T1 T2 -> 
-    DS = nil) /\
-   (forall E q S T, E |= S ~<: T @ q ->  forall T1 T2, T = tp_fun T1 T2 -> 
-    (exists p, exists L, S = tp_sel p L) \/ (exists T1, exists T2, S = tp_and T1 T2) \/ (exists T1, exists T2, S = tp_or T1 T2) \/ (exists TP, exists DS, S = tp_rfn TP DS) \/ 
-    (exists T1', exists T2', S = tp_fun T1' T2' -> exists q, E |= T1 ~<: T1' @ q /\ exists q, E |= T2' ~<: T2 @ q )).
-Proof. 
-mutind_typing P0_ P1_ P2_ P3_ P4_ P5_ P6_ P7_; intros; try solve [inverts H;eauto | inverts H0;eauto | inverts H1;eauto | eauto ].
-
- subst.  admit.
- right. right. right. left. eauto.
- subst. right. right. right. right.
-
-End InvSubFun0.
-
-*)
-
-(*
-Lemma invert_subtyping_and_l : forall E T1 T2 T q, E |= tp_and T1 T2 ~<: T @ q -> 
-  (exists q, E |= T1 ~<: T @ q) /\ (exists q, E |= T2 ~<: T @ q).
-Proof. Admitted.
-
-  mutind_typing P0_ P1_ P2_ P3_ P4_ P5_ P6_ P7_; intros; try solve [ eauto ].
-
-Lemma invert_subtyping_fun: forall E S T U S' T' q1 q2 s,  E |== s ->
-  E |= (tp_fun S T) ~<: U @ q1 -> E |= U ~<: (tp_fun S' T') @ q2 -> (~ has_tp_sel U) ->
-  exists q1, sub_tp E q1 S' S /\ exists q2, sub_tp E q2 T T'.
-Proof. introv. intros HStoTp HSubL. generalize dependent S'. generalize dependent T'. generalize dependent q2.
-  dependent induction HSubL; introv; intros HSubR. (* first get all subgoals to shape  S -> T <: S' -> T' *)
-
-    destruct T0; unfold open_tp in *; simpl in *; inverts x. intros. admit. (* peq *)
-    admit. (* tp_fun does not expand*)
-    intros. set (H2 p L) as HH. unfold not in HH. tauto. (* trans for tp_sel *)
-    intros. assert (tp_fun S T = tp_fun S T); auto. set (@IHHSubL1 S T HStoTp H1 (q2 & q0) T'0 S' (sub_tp_trans H0 HSubL2 HSubR)). auto. (* ok trans: use IH *)
-    intros. admit. (* refl *)
-    intros. admit. (* fun -> do common thing, then use trans*)
-    intros. destruct (invert_subtyping_and_l HSubR) as [HSub1 HSub2]. inverts HSub1. apply IHHSubL1 with (q2 := x); auto. admit. admit. admit. 
-*)
-
-
-(*
-Inductive subsumes_top : env -> tp -> Prop := 
- | st_top : forall E,  subsumes_top E tp_top
- | st_rfn : forall E T, subsumes_top E T -> subsumes_top E (tp_rfn T nil)
- | st_and : forall E T1 T2, subsumes_top E T1 -> subsumes_top E T2 -> subsumes_top E (tp_and T1 T2)
- | st_or1 : forall E T1 T2, subsumes_top E T1 -> subsumes_top E (tp_or T1 T2)
- | st_or2 : forall E T1 T2, subsumes_top E T2 -> subsumes_top E (tp_or T1 T2).
-
-Hint Constructors subsumes_top.
-
-(*
- | st_sel_punt : forall E p L q,
-  E |= tp_top ~<: (tp_sel p L) @ q ->
-  subsumes_top E (tp_sel p L).
- | st_sel_lower : forall E p T' q1 DS q2 L S U,
-  E |= p ~: T' @ q1 ->
-  E |= T' ~< DS @ q2 ->
-  lbl.binds L (decl_tp S U) DS ->
-  path_safe E p ->
-  subsumes_top E (S ^tp^ p) ->
-  subsumes_top E (tp_sel p L)
- | st_sel_upper : forall E p T' q1 DS q2 L S U,
-  E |= p ~: T' @ q1 ->
-  E |= T' ~< DS @ q2 ->
-  lbl.binds L (decl_tp S U) DS ->
-  path p ->
-  subsumes_top E (tp_sel p L) ->
-  subsumes_top E (U ^tp^ p).*)
-
-Lemma opening_pres_subsumes_top : forall E T p p', path_eq E p p' -> subsumes_top E (T ^tp^ p) -> subsumes_top E (T ^tp^ p'). 
-Proof.
-  introv. intros Hpeq H. unfold open_tp in *; simpl. induction T; try solve [inverts H; simpl; auto].
-    simpl in *. inverts H. eapply st_sel; eauto.
-    induction l. simpl. auto. inverts H2.
-Qed.
-
-Lemma and_decls_nil_2 : forall ds, and_decls nil nil ds -> ds = nil.
-Proof. introv. intros.   unfold and_decls in H. destruct H as [_ [HDSOk1 [HDSOk2 H]]]. unfold iff in H. assert (forall (l : label) (d : decl),
-      lbl.binds l d ds ->
-      (exists d1 d2,
-       lbl.binds l d1 nil /\
-       lbl.binds l d2 nil /\ and_decl d1 d2 d) \/
-      lbl.binds l d nil \/ lbl.binds l d nil) by apply H. clear H.
-   induction ds; auto. destruct a. unfold lbl.binds in H0. destruct (H0 l d); simpl; auto.
-   destruct H. destruct H. destruct H. destruct H. 
-   destruct H. destruct H. destruct H. 
-Qed.
-
-Lemma or_decls_nil_2 : forall ds1 ds2 ds, or_decls ds1 ds2 ds -> ds1 = nil \/ ds2 = nil -> ds = nil.
-Proof. Admitted.
-
-Section InvSubTop.
-  Let P0_ (E: env) (q: quality) (t: tm) (T: tp) (H: E  |=  t ~: T  @ q) := True.
-  Let P1_ (E : env) (q : quality) (T : tp) (DS : decls) (H: E |= T ~< DS @ q) := subsumes_top E T -> DS = nil.
-  Let P2_ (E : env) (q : quality) (T T' : tp) (H: E |= T ~<: T' @ q) := subsumes_top E T -> subsumes_top E T'.
-  Let P3_ (e : env) (q : quality) (d d0 : decl) (H: sub_decl e q d d0) := True.
-  Let P4_ (e : env) (t t0 : tm) (H: path_eq e t t0) := True.
-  Let P5_ (e : env) (H: wf_env e) := True.
-  Let P6_ (e : env) (t : tp) (H: wf_tp e t) := True.
-  Let P7_ (e : env) (d : decl) (H: wf_decl e d) := True.
-
-Lemma invert_subtyping_top : 
-   (forall E q T DS, E |= T ~< DS @ q -> E |= T ~<^ T' -> subsumes_top E T -> DS = nil) /\
-   (forall E q T T', E |= T ~<: T' @ q -> subsumes_top E T -> subsumes_top E T').
-Proof. 
-mutind_typing P0_ P1_ P2_ P3_ P4_ P5_ P6_ P7_; intros; try solve [inverts H;eauto | inverts H0;eauto | inverts H1;eauto | eauto ].
-
-(*cases: *)
-    (* expands_rfn *) inverts H0. assert (DSP = nil) by auto. subst. apply and_decls_nil_2; assumption.
-    (* expands_and *) inverts H1. assert (DS1 = nil) by auto; assert (DS2 = nil) by auto. subst. apply and_decls_nil_2; assumption.
-    (* expands_or *) assert (DS1 = nil \/ DS2 = nil) by (inverts H1; [left; auto | right; auto]). apply or_decls_nil_2 with (ds1 := DS1) (ds2 := DS2); assumption.
-    (* sub_tp_rfn_intro *) assert (DS = nil) by auto. subst. inverts H0; auto. 
-    (* sub_tp_rfn *) eauto. assert (DS2 = nil). inverts H. unfold LabelSetImpl.Subset in s. simpl in s. induction DS2; auto. destruct a. assert (LabelSetImpl.In l LabelSetImpl.empty). apply (s l). eapply (lbl.binds_In); eauto. LabelSetDecide.fsetdec. subst. inverts H. auto.
-    (* sub_tp_rfn_precise *) inverts H0; auto.
-      assert (DS2 = nil). unfold LabelSetImpl.Subset in e. simpl in e. induction DS2; auto. destruct a. simpl in e. unfold LabelSetImpl.Equal in e. unfold iff in e. destruct (e l) as [HF _]. assert ( LabelSetImpl.In l LabelSetImpl.empty). LabelSetDecide.fsetdec. rewrite (LabelSetFacts.empty_iff) in H0. contradiction H0. subst. auto.
-    (* sub_tp_tpsel_lower *) 
-    (* sub_tp_tpsel_upper *) 
-    (* sub_tp_path_eq *) apply opening_pres_subsumes_top with (p := p'); auto.
-Qed.
-End InvSubTop.
-
-assert (E |= (S ^tp^ p) ~<: (tp_sel p L) @ subsumed) by (eapply sub_tp_tpsel_lower; eauto). assert (exists q, E |= tp_top ~<: (S ^tp^ p) @ q) as HSubS by admit. destruct HSubS. eapply st_sel_punt. eapply sub_tp_trans; eauto.
-assert (E |= (tp_sel p L) ~<: (U ^tp^ p) @ (q1 & q2)) by (eapply sub_tp_tpsel_upper; eauto). inverts H1 as HSubS. eapply st_sel_punt. eapply sub_tp_trans; eauto.
-*)
-
-
-
-(*
-Reserved Notation "E |= T1 ~<^ T2" (at level 69).
-
-(* chase type member selections up *)
-Inductive promote : env -> tp -> tp -> Prop :=
-  | promote_upper : forall E p T' DS L S U T,
-      E |= p ~: T' @ precise -> E |= T' ~< DS @ precise -> lbl.binds L (decl_tp S U) DS -> (*      path p -> for regularity *)
-      E |= (U ^tp^ p) ~<^ T ->
-      E |= (tp_sel p L) ~<^ T 
-  | promote_lower : forall E p T' DS L S U T,
-      E |= p ~: T' @ precise -> E |= T' ~< DS @ precise -> lbl.binds L (decl_tp S U) DS -> (*      path p -> for regularity *)
-      E |= (U ^tp^ p) ~<^ T ->
-      E |= (S ^tp^ p) ~<^ T
-  | promote_refl : forall E T,
-      (forall p L, T <> (tp_sel p L)) ->
-      E |= T ~<^ T 
-      
-where "E |= T1 ~<^ T2" := (promote E T1 T2).
-
-  Let P1_ (E : env) (q : quality) (T : tp) (DS : decls) (H: E |= T ~< DS @ q) := True. (*exists T1, exists T2, is_fun T T1 T2 -> DS = nil.*)
-  Let P2_ (E : env) (q : quality) (T T' : tp) (H: E |= T ~<: T' @ q) := 
-      (exists p, exists L,   T' = tp_sel p L   -> forall U,     E |= T' ~<^ U -> E |= T ~<^ U) /\
-      (exists S2, exists T2, T' = tp_fun S2 T2 -> forall S1 T1,                  E |= T ~<^ tp_fun S1 T1 -> exists q1, exists q2, E |= S2 ~<: S1 @ q1 /\ E |= T1 ~<: T2 @ q2).
-
-  mutind_typing P0_ P1_ P2_ P3_ P4_ P5_ P6_ P7_; intros; split; try solve [ repeat eexists; discriminate ].
-  repeat eexists. intros. rewrite -> H0 in *.
-Show 5.
-*)
-
-(*
-Lemma and_decls_nil : forall ds1 ds2, and_decls ds1 ds2 nil -> ds1 = nil /\ ds2 = nil.
-Proof. introv. intros. 
-  unfold and_decls in H. destruct H as [_ [HDSOk1 [HDSOk2 H]]]. assert (forall (l : label) (d : decl), (
-      (exists d1 d2, lbl.binds l d1 ds1 /\ lbl.binds l d2 ds2 /\ and_decl d1 d2 d) \/
-       lbl.binds l d ds1 \/ 
-       lbl.binds l d ds2) -> lbl.binds l d nil). unfold iff in H. apply H.  clear H.  
-        unfold lbl.binds in H0. simpl in H0. induction ds1; induction ds2; auto; destruct a. 
-         destruct (H0 l d). right. right. simpl. left. auto.
-         destruct (H0 l d). right. left. simpl. left. auto.
-         destruct (H0 l d). right. left. simpl. left. auto.
-Qed.
-
-
-(*Lemma top_insensitive_opening : forall T p, subsumes_top T -> subsumes_top (T ^tp^ p). 
-Proof.
-  intros. induction H; auto; unfold open_tp in *; simpl; auto.
-Qed.*)
-
-(*Instance EqDec_eq_label : EqDec_eq label.
-Proof. unfold EqDec_eq. decide equality; decide equality; eauto. Defined.
-
-Set Implicit Arguments.
-Lemma binds_map_3 : forall A B (x: label) (b: B) (f: A -> B) E,
-  (forall a b, f a = f b -> a = b) ->
-  lbl.uniq E ->
-  lbl.binds x b (lbl.map f E) ->
-  exists a, lbl.binds x a E /\ b = f a.
-Proof.
-  labelmap induction E; intros HFInjection HUniq HBTail.
-    inversion HBTail. set (lbl.binds_map_1 B A f x b HBTail).
-set (lbl.binds_app_uniq_1 B x b _ _ HUniq HBTail).
-    unfold lbl.binds in *. simpl in *. destruct (x == x0); subst.
-      inverts HUniq. exists a. split. left; auto. inverts HBTail; eauto. inverts H; auto.
-      right. auto.
-Qed.*)
-
-Inductive not_lambda : tm -> Prop :=
-| not_lambda_bvar : forall x, not_lambda (bvar x)
-| not_lambda_fvar : forall x, not_lambda (fvar x)
-| not_lambda_ref  : forall x, not_lambda (ref x)
-| not_lambda_app  : forall x y, not_lambda (app x y)
-| not_lambda_new  : forall x y z, not_lambda (new x y z)
-| not_lambda_sel  : forall x y, not_lambda (sel x y).
-Hint Constructors not_lambda.
-
-(* the hard case is T = tp_rfn TP DS -- need to appeal to a more powerful lemma that says that expansion is monotone under subtyping *)  
-Lemma lambdas_dont_have_members: forall E t T q1 DS q2,  E |= t ~: T @ q1 -> E |= T ~< DS @ q2 -> DS <> nil -> not_lambda t.
-Proof. 
-  introv HT HX HNotNil. generalize dependent q1. generalize dependent t. 
-  induction HX; intros; 
-    try (inverts HT; eapply (IHHX _ _ _ (typing_sub _ H)); eauto); 
-    try tauto. 
-  
-  destruct t; auto.
-
-*)
-
-(* false: does not work when e.l -> e'.l -- the IH says e' may still be a lambda 
-Lemma path_red_path_or_lambda: forall s t t' s', path t -> s |~ t ~~> t' ~| s' -> path t' \/ (exists T, exists tb, t' = lam T tb).
-Proof.
-  intros. induction H0; inverts H; eauto. inverts H2; auto. right; eauto. set (IHred H2) as IH. left.
-*)
-
-(*
-Lemma invert_typing_sel : forall E S t U q, E |= sel t l ~: T @ q -> exists q0, exists q1, exists T, E |= lam S t ~: (tp_fun S T) @ q0 /\ sub_tp E q1 (tp_fun S T) U.
-Admitted.
-*)
-(*
-Lemma and_decls_nil: and_decls nil nil nil.
-Proof. Admitted.
-
-Lemma and_decls_nil_1: forall DS, and_decls nil DS DS.
-Proof. Admitted.
-
-Lemma and_decls_nil_2: forall DS, and_decls DS nil DS.
-Proof. Admitted.
-
-Lemma or_decls_nil: or_decls nil nil nil.
-Proof. Admitted.
-
-Lemma or_decls_nil_1: forall DS, or_decls nil DS nil.
-Proof. Admitted.
-
-Lemma or_decls_nil_2: forall DS, or_decls DS nil nil.
-Proof. Admitted.
-
-Lemma invert_and_decls_nil_1: forall DS DS', and_decls nil DS DS' -> DS = DS'.
-Proof. Admitted.
-Lemma invert_and_decls_nil_2: forall DS DS', and_decls DS nil DS' -> DS = DS'.
-Proof. Admitted. 
-
-Hint Rewrite invert_and_decls_nil_1 invert_and_decls_nil_2 : decls.
-*)
 (*
 *** Local Variables: ***
 *** coq-prog-name: "coqtop" ***
